Golfed a few lines, planned TFAE theorem

FormalizationOfComputability/PhiSeq.lean
@@ -22,7 +22,7 @@ open List --hiding isSome_getElem?
 /- The elements whose computations first halt at stage s, in increasing order. By definition,
 these elements are less than s. -/
 def PhiNewList (e s : ℕ) : List ℕ :=
-  (range s).filter (λ n => (Phi_s_halts e s n ∧ ¬ Phi_s_halts e (s-1) n))
+  (range s).filter (λ n ↦ (Phi_s_halts e s n ∧ ¬ Phi_s_halts e (s-1) n))
 
 def PhiNew (e s : ℕ) : Finset ℕ := (PhiNewList e s).toFinset
 
@@ -31,9 +31,13 @@ lemma PhiNewList_zero (e : ℕ) : PhiNewList e 0 = ∅ := by
 
 /- A helper lemma for moving between the list and set forms-/
 lemma PhiNewList_mem (e s x : ℕ) : x ∈ PhiNewList e s ↔ x ∈ PhiNew e s := by
-  constructor
-  · simp [PhiNewList, PhiNew]
-  · simp [PhiNew]
+  simp [PhiNewList, PhiNew]
+
+/- This lemma cleans up lines that would otherwise be a rather lengthy simp only -/
+private
+lemma PhiNew_mem_lemma (e s x : ℕ) :
+    x ∈ PhiNew e s ↔ (x < s ∧ Phi_s_halts e s x ∧ ¬Phi_s_halts e (s - 1) x) := by
+  simp [PhiNew, PhiNewList]
 
 /- The elements newly halting at stage s are exactly W_{e, s} \ W_{e, s-1} -/
 lemma PhiNew_eq_Ws_diff (e s : ℕ) : (PhiNew e s) = (W_s e s) \ (W_s e (s-1)) := by
@@ -42,13 +46,17 @@ lemma PhiNew_eq_Ws_diff (e s : ℕ) : (PhiNew e s) = (W_s e s) \ (W_s e (s-1)) :
   · intro x
     simp_all [PhiNewList]
   · intro x
-    simp
+    simp only [Finset.mem_sdiff, Finset.mem_filter, Finset.mem_range, not_and, mem_toFinset,
+      and_imp]
     intro h1 h2 h3
-    simp_all [PhiNewList]
-    contrapose h3
-    simp_all
-    have h4 : x < s - 1 := by exact halt_input_bound e (s-1) x h3
-    exact add_lt_of_lt_sub h4
+    simp [PhiNewList]
+    constructor
+    · exact h1
+    · simp_all only [true_and]
+      contrapose h3
+      simp_all only [Classical.not_imp, Decidable.not_not]
+      have h4 := halt_input_bound e (s-1) x h3
+      simp only [h4, and_self]
 
 /- Elements never enter twice - the PhiNew are disjoint -/
 lemma PhiNew_disjoint_gt (e s t : ℕ) (h : s > t) :
@@ -57,9 +65,7 @@ lemma PhiNew_disjoint_gt (e s t : ℕ) (h : s > t) :
   simp [PhiNew, PhiNewList]
   intro a _ _ h1 b _ h2 _
   contrapose h1
-  simp
-  simp at h1
-  simp [← h1] at h2
+  simp_all only [Decidable.not_not]
   apply phi_halts_mono e t
   · cases' s with s
     · tauto
@@ -82,7 +88,7 @@ lemma PhiNew_is_new (e s : ℕ) : (PhiNew e s) ∩ (W_s e (s-1)) = ∅ := by
 /- It is sometimes useful to work with W_{e,s} instead of W_{e, s+1} -/
 lemma Ws_eq (e s : ℕ) : W_s e s = (W_s e (s-1)) ∪ (PhiNew e s) := by
     rw [PhiNew_eq_Ws_diff]
-    simp
+    simp only [Finset.union_sdiff_self_eq_union, Finset.right_eq_union]
     apply W_s_mono
     simp
 
@@ -91,7 +97,7 @@ lemma PhiNew_runtime_iff (e x r : ℕ) : x ∈ PhiNew e r ↔ r ∈ runtime e x 
   constructor
   <;> intro h
   · rw [runtime_is_min]
-    simp [PhiNew, PhiNewList] at h
+    rw [PhiNew_mem_lemma] at h
     constructor
     · exact h.right.left
     · intro t h1
@@ -115,8 +121,7 @@ lemma PhiNew_runtime_iff (e x r : ℕ) : x ∈ PhiNew e r ↔ r ∈ runtime e x 
       apply Nat.ne_zero_of_lt at h2
       cases' r with r
       · tauto
-      · simp
-        rw [← Phi_s_diverges]
+      · simp only [add_tsub_cancel_right]
         apply h.right
         linarith
 
@@ -124,63 +129,19 @@ lemma PhiNew_runtime_iff (e x r : ℕ) : x ∈ PhiNew e r ↔ r ∈ runtime e x 
 lemma We_eq_union_WsNew (e : ℕ) : W e = ⋃ s, (PhiNew e s) := by
   rw [W_eq_union_W_s]
   apply subset_antisymm
-  · intro x h
-    simp at h
-    obtain ⟨s, h⟩ := h
+  <;> intro x h
+  <;> simp_all only [Set.mem_iUnion, Finset.mem_coe]
+  · obtain ⟨_, h⟩ := h
     apply Ws_runtime at h
-    obtain ⟨r, ⟨h, h1⟩⟩ := h
-    simp
+    obtain ⟨r, h⟩ := h
     use r
     rw [PhiNew_runtime_iff]
-    exact h
-  · intro x h
-    simp at h
-    obtain ⟨s, h⟩ := h
-    rw [PhiNew_eq_Ws_diff] at h
-    simp
-    use s
-    simp at h
     exact h.left
-
-/- If eventually no new elements ever enter, then W_{e, s} never again changes-/
-lemma WsNew_stabilizes_Ws_stabilizes (e t : ℕ) (h : ∀ s ≥ t, PhiNew e s = ∅) :
-    ∀ s ≥ t, W_s e s = W_s e t := by
-  have h1 : ∀ s ≥ t, (W_s e (s+1)) = (W_s e s) := by
-    intro s h1
-    rw [Ws_eq]
-    simp
-    have h2 : PhiNew e (s+1) = ∅ := by
-      apply h
-      linarith
-    rw [h2]
-    simp
-  intro s h2
-  induction' s using Nat.strong_induction_on with s ih
-  by_cases h3 : s = t
-  · simp [h3]
-  · have h4 : s-1 ≥ t := by
-      refine le_sub_one_of_lt ?_
-      exact Nat.lt_of_le_of_ne h2 fun a ↦ h3 (id (Eq.symm a))
-    have h5 : (W_s e (s-1)) = (W_s e t) := by
-      apply ih (s-1)
-      · apply Nat.sub_one_lt
-        cases t
-        · tauto
-        · linarith
-      exact h4
-    rw [← h5]
-    have h6 : W_s e ((s - 1) + 1) = (W_s e (s-1)) := by
-      exact h1 (s - 1) h4
-    have h7 : s - 1 + 1 = s := by
-      refine Nat.sub_add_cancel ?_
-      cases t
-      · exact one_le_iff_ne_zero.mpr h3
-      · exact one_le_of_lt h2
-    rw [h7] at h6
-    exact h6
-
-
-
+  · obtain ⟨s, h⟩ := h
+    rw [PhiNew_eq_Ws_diff] at h
+    use s
+    simp only [Finset.mem_sdiff] at h
+    exact h.left
 
 /- TFAE :
 Eventually all PhiNew e s = ∅
@@ -192,113 +153,66 @@ There is an s such that W_e = W_{e, s}
 lemma PhiNew_stabilizes_implies_We_finite (e s : ℕ) (h : ∀ t > s, PhiNew e t = ∅) :
     (W e).Finite := by
   rw [We_eq_union_WsNew, Set.finite_iUnion_iff]
-  · simp
+  · simp only [Finset.finite_toSet, implies_true, Finset.coe_nonempty, true_and]
     apply Set.Finite.subset (Set.finite_le_nat s)
-    simp
+    simp only [Set.setOf_subset_setOf]
     intro t h1
     contrapose h1
     simp_all
-  · simp
+  · simp only [Finset.disjoint_coe]
     intro i j h1
     apply PhiNew_pairwise_disjoint
-    <;> simp
+    <;> simp only [Set.mem_univ, ne_eq]
     exact h1
-
-lemma PhiNew_stabilizes_implies_We_eq_Ws (e s : ℕ) (h : ∀ t > s, PhiNew e t = ∅) :
-    W e = W_s e s := by
-  rw [We_eq_union_WsNew]
-  apply subset_antisymm
-  · intro x h1
-    simp at h1
-    obtain ⟨r, h1⟩ := h1
-    have h2 : r ≤ s := by
-      contrapose h1
-      simp at h1
-      apply h at h1
-      rw [h1]
-      simp
-    have h3 : x ∈ W_s e r := by
-      rw [Ws_eq]
-      exact Finset.mem_union_right (W_s e (r - 1)) h1
-    apply W_s_mono e r
-    · exact h2
-    · exact h3
-  · intro x h1
-    apply Ws_runtime at h1
-    obtain ⟨r, ⟨h1, h2⟩⟩ := h1
-    rw [← PhiNew_runtime_iff] at h1
-    simp
-    use r
 
 lemma We_finite_implies_PhiNew_stabilizes (e : ℕ) (h : (W e).Finite) :
     ∃ s, ∀ t > s, PhiNew e t = ∅ := by
   rw [We_eq_union_WsNew, Set.finite_iUnion_iff] at h
-  simp at h
-  have h1 :  ∃ P : Finset ℕ, ∀ n, n ∈ P ↔ n ∈ {i | (PhiNew e i).Nonempty} := by
-    apply Set.Finite.exists_finset h
+  simp only [Finset.finite_toSet, implies_true, Finset.coe_nonempty, true_and] at h
+  have h1 := Set.Finite.exists_finset h
   obtain ⟨P, h1⟩ := h1
   · by_cases h2 : P = ∅
     · use 0
-      intro s h3
-      rw [h2] at h1
-      simp at h1
-      apply h1
-    · let N := Finset.max' P (Finset.nonempty_iff_ne_empty.mpr h2)
-      use N
+      simp_all
+    · use Finset.max' P (Finset.nonempty_iff_ne_empty.mpr h2)
       intro s h3
       contrapose h3
-      simp
-      push_neg at h3
-      have h4 : s ∈ P := by
-        rw [h1]
-        simp
-        exact Finset.nonempty_iff_ne_empty.mpr h3
-      simp [lt_iff_add_one_le]
-      exact Finset.le_max' P s h4
-  · simp
+      simp only [gt_iff_lt, Finset.max'_lt_iff, not_forall, Classical.not_imp, not_lt]
+      use s
+      simp only [le_refl, exists_prop, and_true, h1, Set.mem_setOf_eq]
+      exact Finset.nonempty_iff_ne_empty.mpr h3
+  · simp only [Finset.disjoint_coe]
     intro i j h1
     apply PhiNew_pairwise_disjoint
-    <;> simp
+    <;> simp only [Set.mem_univ, ne_eq]
     exact h1
 
 lemma We_finite_iff_PhiNew_stabilizes (e : ℕ) :
     (W e).Finite ↔ (∃ t, ∀ s > t, PhiNew e s = ∅) := by
   constructor
-  · apply We_finite_implies_PhiNew_stabilizes e
-  · intro ⟨t, h⟩
+  · exact We_finite_implies_PhiNew_stabilizes e
+  · intro ⟨_, h⟩
     apply PhiNew_stabilizes_implies_We_finite
     exact h
-
-lemma We_finite_iff_We_eq_Ws (e : ℕ) : (W e).Finite ↔ ∃ s, W e = W_s e s := by
-  constructor
-  · rw [We_finite_iff_PhiNew_stabilizes]
-    intro ⟨t, h⟩
-    use t
-    apply PhiNew_stabilizes_implies_We_eq_Ws
-    exact h
-  · intro ⟨s, h⟩
-    rw [h]
-    simp
 
 /- x appears as a new element at its runtime -/
 lemma PhiNew_runtime (y e s : ℕ) : y ∈ PhiNew e s ↔ s ∈ runtime e y := by
   simp [runtime, rfindOpt]
   constructor
-  · simp [PhiNew, PhiNewList, W_s]
-    intro h h1 h2
+  <;> simp_all only [PhiNew_mem_lemma]
+  · intro ⟨h, ⟨h1, h2⟩⟩
     constructor
-    · exact Option.isSome_iff_exists.mpr h1
+    · obtain ⟨x, h1⟩ := h1
+      exact Option.isSome_of_mem h1
     · intro m hm
-      have h3 : Phi_s_halts e s y → y < s := by
-        apply halt_input_bound
+      have h3 := halt_input_bound e s y
       apply phi_halts_mono_reverse e m at h2
-      · unfold Phi_s_diverges Phi_s_halts at h2
+      · unfold Phi_s_halts at h2
         push_neg at h2
         exact Option.eq_none_iff_forall_ne_some.mpr h2
       · exact le_sub_one_of_lt hm
   · intro ⟨h, h1⟩
     apply Option.isSome_iff_exists.mp at h
-    simp [PhiNew, PhiNewList]
     constructor
     · apply halt_input_bound e
       simp [Phi_s_halts, h]
@@ -306,7 +220,7 @@ lemma PhiNew_runtime (y e s : ℕ) : y ∈ PhiNew e s ↔ s ∈ runtime e y := b
       · exact h
       · unfold Phi_s_halts
         push_neg
-        intro y
+        intro x
         by_cases h2 : s=0
         · simp [h2, Phi_s]
         · simp [h1, sub_one_lt, h2]
@@ -319,30 +233,29 @@ def WPrefix (e : ℕ) : ℕ → List ℕ
 /- WPrefix e s is exactly W_{e, s} in order of enumeration -/
 lemma Ws_eq_prefix (e s : ℕ) : W_s e s = (WPrefix e s).toFinset := by
   induction' s with s hs
-  · simp [WPrefix, W_s]
+  · simp only [W_s, Finset.range_zero, Finset.filter_empty, WPrefix, toFinset_nil]
   · apply subset_antisymm
     intro y h
-    simp [WPrefix]
+    simp only [WPrefix, toFinset_append, Finset.mem_union, mem_toFinset]
     by_cases h1 : y ∈ (W_s e s)
     · left
       rw [← mem_toFinset, ← hs]
       exact h1
     · right
-      simp [PhiNew, PhiNewList]
+      simp only [PhiNewList_mem, PhiNew_mem_lemma]
       simp [W_s] at h
       constructor
       · exact h.left
       · constructor
         · exact h.right
-        · have h2 : Phi_s_halts e s y → y < s := by
-            apply halt_input_bound
-          simp [W_s] at h1
+        · have h2 := halt_input_bound e s y
+          simp only [W_s, Finset.mem_filter, Finset.mem_range, not_and] at h1
           tauto
     · intro x h
       simp [WPrefix, PhiNew, W_s] at h
       rw [PhiNewList_mem, ← mem_toFinset, ← hs] at h
-      simp [W_s]
-      simp [W_s] at h
+      simp only [W_s, Finset.mem_filter, Finset.mem_range]
+      simp only [W_s, Finset.mem_filter, Finset.mem_range] at h
       rcases h with h | h
       · constructor
         · linarith
@@ -350,10 +263,10 @@ lemma Ws_eq_prefix (e s : ℕ) : W_s e s = (WPrefix e s).toFinset := by
           · linarith
           · exact h.right
       · rw [PhiNew_eq_Ws_diff] at h
-        simp [W_s] at h
+        simp only [W_s, add_tsub_cancel_right, Finset.mem_sdiff, Finset.mem_filter,
+          Finset.mem_range, not_and] at h
         constructor
-        · exact h.left.left
-        · exact h.left.right
+        <;> simp [h]
 
 lemma WPrefix_mem (e s n : ℕ) : n ∈ WPrefix e s ↔ n ∈ W_s e s := by
   rw [← mem_toFinset, Ws_eq_prefix]
@@ -369,27 +282,26 @@ lemma nodup_WPrefix (e s : ℕ) : Nodup (WPrefix e s) := by
   induction' s with s ih
   · unfold WPrefix
     simp
-  · simp [WPrefix]
+  · simp only [WPrefix]
     apply List.Nodup.append
     · exact ih
     · apply List.Nodup.filter
       exact nodup_range
     · unfold List.Disjoint
-      intro a h h1
-      simp [PhiNewList_mem, PhiNew_eq_Ws_diff, Ws_eq_prefix] at h1
-      obtain ⟨h1, h2⟩ := h1
+      intro _ _ h1
+      simp only [PhiNewList_mem, PhiNew_eq_Ws_diff, Ws_eq_prefix, add_tsub_cancel_right,
+        Finset.mem_sdiff, mem_toFinset] at h1
       tauto
 
 /- The WPrefixes are prefixes of each other-/
 lemma WPrefix_mono (e s t : ℕ) (h : s ≤ t) :
   (WPrefix e s) <+: (WPrefix e t) := by
   induction' t with t ih
-  · simp at h
+  · simp only [nonpos_iff_eq_zero] at h
     rw [h]
   · by_cases h1 : s = t + 1
     · rw [h1]
-    · have h2 : s ≤ t := by
-        exact le_of_lt_succ (lt_of_le_of_ne h h1)
+    · have h2 : s ≤ t := le_of_lt_succ (lt_of_le_of_ne h h1)
       apply ih at h2
       apply List.IsPrefix.trans h2
       simp [WPrefix]
@@ -423,8 +335,7 @@ lemma enter_queue_halts (e s n: ℕ) (h : n ∈ enter_queue e s) : Phi_s_halts e
     · apply List.mem_of_mem_tail at h
       apply ih at h
       exact phi_halts_mono e s (s+1) n (Nat.le_add_right s 1) h
-    · simp [PhiNewList] at h
-      exact h.right.left
+    · simp_all only [PhiNewList_mem, PhiNew_mem_lemma]
 
 /- Elements of the queue are exactly the elements that halt -/
 lemma enter_queue_mem (e n : ℕ) : (∃ s, n ∈ enter_queue e s) ↔ Phi_halts e n := by
@@ -434,35 +345,34 @@ lemma enter_queue_mem (e n : ℕ) : (∃ s, n ∈ enter_queue e s) ↔ Phi_halts
     apply (phi_halts_stage_exists e n).mpr
     use s
   · intro h
-    simp [phi_halts_runtime_exists, ← PhiNew_runtime_iff] at h
+    simp only [phi_halts_runtime_exists, ← PhiNew_runtime_iff] at h
     obtain ⟨r, h⟩ := h
     use r
     unfold enter_queue
     cases' r with r
     · tauto
-    · simp
+    · simp only [mem_append]
       right
       simp [PhiNewList_mem, h]
 
 /- A lemma for moving from (enter_queue e s) to (enter_queue e t) -/
 lemma enter_queue_PhiNewList (e t s : ℕ) (h : s ≥ t) :
     (enter_queue e s) <:+
-    (enter_queue e t) ++ flatten ((range (s - t)).map (λ i => PhiNewList e (t + i + 1))) := by
+    (enter_queue e t) ++ flatten ((range (s - t)).map (λ i ↦ PhiNewList e (t + i + 1))) := by
   apply Nat.exists_eq_add_of_le at h
   obtain ⟨k, h⟩ := h
   revert s
   induction' k with k ih
   · simp_all
-  · simp_all
+  · simp_all only [add_tsub_cancel_left, forall_eq]
     rw [← add_assoc]
-    dsimp [enter_queue]
+    simp only [enter_queue]
     rw [List.range_succ]
     have ih1 : (enter_queue e (t + k)).tail <:+
     enter_queue e t ++ (map (fun i ↦ PhiNewList e (t + i + 1)) (range k)).flatten := by
       apply IsSuffix.trans
       apply List.tail_suffix
       exact ih
-    clear ih
     have ih2 : (enter_queue e (t + k)).tail ++ PhiNewList e (t + k + 1) <:+
     (enter_queue e t ++
     (map (fun i ↦ PhiNewList e (t + i + 1)) (range k)).flatten) ++ PhiNewList e (t + k + 1) := by
@@ -472,24 +382,24 @@ lemma enter_queue_PhiNewList (e t s : ℕ) (h : s ≥ t) :
     simp_all
 
 /- The queue at stage s is a suffix of WPrefix e s.
-This is mostly here to make the next lemma easy -/
+This is mostly here so that it's easy to show that enter queues have no duplicates -/
 lemma enter_queue_WPrefix (e s : ℕ) :
     IsSuffix (enter_queue e s) (WPrefix e s) := by
   induction' s with s ih
   · simp [enter_queue]
   · unfold enter_queue WPrefix
-    have h1 : (enter_queue e s).tail <:+ WPrefix e s := by
-      apply List.IsSuffix.trans (tail_suffix (enter_queue e s)) ih
+    have h1 : (enter_queue e s).tail <:+ WPrefix e s :=
+      List.IsSuffix.trans (tail_suffix (enter_queue e s)) ih
     cases' L : (enter_queue e s) with a T
     · simp
-    · simp [L, IsSuffix] at h1
+    · simp only [IsSuffix, L, tail_cons] at h1
       obtain ⟨S, h1⟩ := h1
       use S
       simp [← h1]
 
 /- The queues have no duplicates. -/
 lemma enter_queue_nodup (e s : ℕ) : Nodup (enter_queue e s) := by
-  have ⟨L, h⟩ := enter_queue_WPrefix e s
+  have ⟨_, h⟩ := enter_queue_WPrefix e s
   have h1 := nodup_WPrefix e s
   rw [← h] at h1
   exact List.Nodup.of_append_right h1
@@ -509,17 +419,14 @@ lemma enter_queue_nodup_elements (e s k i n : ℕ) (h : (enter_queue e s)[k]? = 
 lemma enter_queue_dec_stage (e n s : ℕ)
     (h : n ∈ (enter_queue e s).tail) :
      List.idxOf? n (enter_queue e (s + 1)) = (List.idxOf? n (enter_queue e s)).map (· - 1) := by
-  dsimp [enter_queue]
-  simp [List.idxOf?_append, h]
+  simp only [enter_queue, idxOf?_append, h, ↓reduceIte]
   cases' hL : enter_queue e s with a T
   · tauto
-  · simp
+  · simp only [tail_cons]
     rw [index_tail] at h
     obtain ⟨k, ⟨h, h1⟩⟩ := h
     rw [← idxOf?_getElem?_iff] at h1
-    · rw [hL] at h1
-      rw [← h1]
-      simp
+    · simp_all only [Option.map_some]
       have h3 : some k = idxOf? n ([a] ++ T) := by exact h1
       rw [List.idxOf?_append] at h3
       have h4 : n ∈ (a :: T).tail := by
@@ -528,17 +435,17 @@ lemma enter_queue_dec_stage (e n s : ℕ)
         use k
       have h5 : n ≠ a := by
         contrapose h
-        simp at h
-        simp
-        have h2 := idxOf?_length h1
-        apply List.getElem?_inj h2
+        simp only [ne_eq, Decidable.not_not] at h
+        simp only [ge_iff_le, not_le, lt_one_iff]
+        apply List.getElem?_inj (idxOf?_length h1)
         · rw [← hL]
           exact enter_queue_nodup e s
         · rw [idxOf?_getElem? h1]
           simp [h]
       apply index_tail_minus_one at h4
-      simp [h5, ← h1] at h4
-      exact h4
+      simp only [head?_cons, Option.some.injEq, h5, tail_cons, ← h1, Option.map_some,
+        false_or] at h4
+      simp [← h1, h4]
     · have h3 := enter_queue_nodup e s
       intro i hik
       apply enter_queue_nodup_elements e s k i n h1
@@ -559,7 +466,7 @@ lemma enter_queue_dec (e n s k l : ℕ) (h : List.idxOf? n (enter_queue e s) = s
   · intro n hn hk
     have ⟨h3, h4⟩ : n ∈ enter_queue e (s + l) ∧ idxOf? n (enter_queue e (s + l)) = some (k - l) := by
       apply ih (le_of_succ_le h1)
-      simp_all
+      simp_all only [mem_cons, forall_eq_or_imp]
       exact hk
     have h5 : n ∈ (enter_queue e (s + l)).tail := by
       rw [index_tail]
@@ -582,18 +489,17 @@ lemma enter_queue_enum_exact (e s n k : ℕ) (h : List.idxOf? n (enter_queue e s
   have h1 : k ≤ k := by rfl
   apply enter_queue_dec at h
   apply h at h1
-  simp at h1
-  obtain ⟨h1, h2⟩ := h1
+  simp only [tsub_self] at h1
+  obtain ⟨_, h1⟩ := h1
   rw [eq_comm, new_element, index_head, ← idxOf?_getElem?_iff]
-  · exact id (Eq.symm h2)
+  · exact id (Eq.symm h1)
   · tauto
 
 /- If n is in a queue, it is eventually enumerated -/
 lemma enter_queue_enum (e s n : ℕ) (h : n ∈ (enter_queue e s)) :
     ∃ t, new_element e t = n := by
-  have ⟨k, h1⟩ : ∃ k, List.idxOf? n (enter_queue e s) = some k := by
-    refine Option.isSome_iff_exists.mp ?_
-    exact isSome_idxOf?.mpr h
+  have ⟨k, h1⟩ : ∃ k, List.idxOf? n (enter_queue e s) = some k :=
+    Option.isSome_iff_exists.mp (isSome_idxOf?.mpr h)
   apply enter_queue_enum_exact at h1
   use s+k
 
@@ -603,7 +509,7 @@ lemma enter_queue_exit_exact (e s n k : ℕ) (h : List.idxOf? n (enter_queue e s
   intro t
   have h1 := idxOf?_mem (id (Eq.symm h))
   have h2 := enter_queue_enum_exact e s n k h
-  have ⟨r, ⟨h3, h4⟩⟩ := runtime_is_min' e s n (enter_queue_halts e s n h1)
+  have ⟨r, ⟨h3, _⟩⟩ := runtime_is_min' e s n (enter_queue_halts e s n h1)
   rw [← PhiNew_runtime_iff] at h3
   induction' t with t ih
   <;> nth_rw 1 [enter_queue]
@@ -611,33 +517,32 @@ lemma enter_queue_exit_exact (e s n k : ℕ) (h : List.idxOf? n (enter_queue e s
   · constructor
     · cases' hL : enter_queue e (s+k) with a T
       · simp_all
-      · have h3 := enter_queue_nodup e (s+k)
-        have h4 := enter_queue_enum_exact e s n k h
-        unfold new_element at h4
+      · have h4 := enter_queue_nodup e (s+k)
+        have h5 := enter_queue_enum_exact e s n k h
+        unfold new_element at h5
         simp_all
-    · have h5 : Disjoint (PhiNew e r) (PhiNew e (s+k+1)) := by
+    · have h4 : Disjoint (PhiNew e r) (PhiNew e (s+k+1)) := by
         refine Disjoint.symm (PhiNew_disjoint_gt e (s + k + 1) r ?_)
         linarith
-      rw [Finset.disjoint_left] at h5
+      rw [Finset.disjoint_left] at h4
       rw [PhiNewList_mem]
-      apply h5 h3
+      exact h4 h3
   · constructor
     · contrapose ih
-      simp_all
+      simp_all only [Decidable.not_not]
       exact mem_of_mem_tail ih
-    · have h5 : Disjoint (PhiNew e r) (PhiNew e (s+k+t+2)) := by
+    · have h4 : Disjoint (PhiNew e r) (PhiNew e (s+k+t+2)) := by
         refine Disjoint.symm (PhiNew_disjoint_gt e (s+k+t+2) r ?_)
         linarith
-      rw [Finset.disjoint_left] at h5
+      rw [Finset.disjoint_left] at h4
       rw [PhiNewList_mem]
-      apply h5 h3
+      exact h4 h3
 
 /- If n is in a queue, eventually it is never in a queue again -/
 lemma enter_queue_exit (e s n : ℕ) (h : n ∈ (enter_queue e s)) :
     ∃ s₁, ∀ t > s₁, n ∉ enter_queue e t := by
-  have ⟨k, h1⟩ : ∃ k, List.idxOf? n (enter_queue e s) = some k := by
-    refine Option.isSome_iff_exists.mp ?_
-    exact isSome_idxOf?.mpr h
+  have ⟨k, h1⟩ : ∃ k, List.idxOf? n (enter_queue e s) = some k :=
+    Option.isSome_iff_exists.mp (isSome_idxOf?.mpr h)
   apply enter_queue_exit_exact at h1
   use s+k+1
   intro t₁ ht1
@@ -661,19 +566,19 @@ lemma Phi_halts_Wenum (e n : ℕ) : Phi_halts e n ↔ ∃ s, n = Wenum e s := by
     use s
     exact mem_of_mem_head? h.symm
 
+/-- TODO: prove a constructive version, then generalize to exists -/
 /- If PhiNew stabilizes, then eventually the queue depletes.
 Indeed iff is true, see TFAE below. -/
 lemma queue_depletes (e : ℕ) (h : (W e).Finite) :
     ∃ t, ∀ s > t, enter_queue e s = [] := by
   rw [We_finite_iff_PhiNew_stabilizes] at h
   obtain ⟨t, h⟩ := h -- unfortunately the queue at stage t may not be empty
-  let l := (enter_queue e t).length
-  use t+l
-  intro s hs
+  use t+(enter_queue e t).length
+  intro s _
   have hx : ∀ x, x ∈ enter_queue e t → x ∉ enter_queue e s := by
     intro x h
     have ⟨k, hxk⟩ := Option.isSome_iff_exists.mp (isSome_idxOf?.mpr h)
-    have hkl : k < l := idxOf?_length hxk.symm
+    have hkl := idxOf?_length hxk.symm
     apply enter_queue_exit_exact at hxk
     have ⟨k1, hsk1⟩ : ∃ k1, s = t + k + k1 + 1 := by
       apply Nat.exists_eq_add_of_lt
@@ -690,11 +595,11 @@ lemma queue_depletes (e : ℕ) (h : (W e).Finite) :
     intro i
     rw [← toFinset_eq_empty_iff]
     exact hi i
-  simp_all
+  simp_all only [gt_iff_lt, ge_iff_le, map_const', length_range, flatten_replicate_nil, append_nil]
   apply IsSuffix.subset at hs1
   rw [← toFinset_eq_empty_iff]
   ext x
-  simp
+  simp only [mem_toFinset, Finset.notMem_empty, iff_false]
   intro h
   have h1 := hs1 h
   apply hx at h1
@@ -706,18 +611,17 @@ lemma Wenum_finite_iff (e : ℕ) : (W e).Finite ↔ ∃ s, ∀ t > s, Wenum e t 
     have ⟨s, h1⟩ := queue_depletes e h
     use s
     intro t ht
-    simp [Wenum, new_element]
-    simp_all
+    simp_all only [Wenum, new_element, head?_eq_none_iff, gt_iff_lt]
   · rw [We_finite_iff_PhiNew_stabilizes]
     intro ⟨t, h⟩
     use t
     intro s h1
-    simp [Wenum, new_element] at h
+    simp only [gt_iff_lt, Wenum, new_element, head?_eq_none_iff] at h
     have h2 : enter_queue e s = [] := by simp_all
     unfold enter_queue at h2
     cases' s with s
     · tauto
-    · simp at h2
+    · simp only [append_eq_nil_iff] at h2
       ext x
       rw [← PhiNewList_mem]
       simp [h2]
@@ -729,12 +633,94 @@ lemma Wenum_infinite_iff (e : ℕ) : (W e).Infinite ↔ ∀ s, ∃ t > s, ∃ n,
 
 
 theorem We_finite_TFAE (e : ℕ) :
-  [
-    (W e).Finite,
-    ∃ s, ∀ t > s, PhiNewList e t = [],
-    ∃ s, ∀ t > s, W_s e t = W_s e s,
-    ∃ s, W e = W_s e s,
-    ∃ s, ∀ t > s, enter_queue e t = [],
-    ∃ s, ∀ t > s, Wenum e t = Option.none
-  ].TFAE := by
+    [
+      (W e).Finite,                         --1
+      ∃ s, ∀ t ≥ s, PhiNew e t = ∅,         --2
+      ∃ s, ∀ t ≥ s, W_s e t = W_s e s,      --3
+      ∃ s, W e = W_s e s,                   --4
+      ∃ s, ∀ t ≥ s, enter_queue e t = [],   --5
+      ∃ s, ∀ t ≥ s, Wenum e t = Option.none --6
+    ].TFAE := by
   sorry
+
+/- Proven above:
+1 ↔ 2 We_finite_iff_PhiNew_stabilizes
+1 → 5 queue_depletes (with s and t switched)
+1 ↔ 6 Wenum_finite_iff
+-/
+
+-- 1 ↔ 2 ↔ 6 ↔ 4 → 3, 5
+-- needed: 3 → 4, 5 → 6
+
+-- 2 → 4
+lemma PhiNew_stabilizes_implies_We_eq_Ws (e s : ℕ) (h : ∀ t > s, PhiNew e t = ∅) :
+    W e = W_s e s := by
+  rw [We_eq_union_WsNew]
+  apply subset_antisymm
+  <;> intro x h1
+  · simp only [Set.mem_iUnion, Finset.mem_coe] at h1
+    obtain ⟨r, h1⟩ := h1
+    have h2 : r ≤ s := by
+      contrapose h1
+      simp only [not_le] at h1
+      apply h at h1
+      rw [h1]
+      simp
+    have h3 : x ∈ W_s e r := by
+      rw [Ws_eq]
+      exact Finset.mem_union_right (W_s e (r - 1)) h1
+    apply W_s_mono e r
+    · exact h2
+    · exact h3
+  · apply Ws_runtime at h1
+    obtain ⟨r, ⟨h1, h2⟩⟩ := h1
+    rw [← PhiNew_runtime_iff] at h1
+    simp only [Set.mem_iUnion, Finset.mem_coe]
+    use r
+
+-- 1 ↔ 4
+lemma We_finite_iff_We_eq_Ws (e : ℕ) : (W e).Finite ↔ ∃ s, W e = W_s e s := by
+  constructor
+  · rw [We_finite_iff_PhiNew_stabilizes]
+    intro ⟨t, h⟩
+    use t
+    apply PhiNew_stabilizes_implies_We_eq_Ws
+    exact h
+  · intro ⟨s, h⟩
+    rw [h]
+    simp
+
+-- 2 → 3
+lemma WsNew_stabilizes_Ws_stabilizes (e t : ℕ) (h : ∀ s ≥ t, PhiNew e s = ∅) :
+    ∀ s ≥ t, W_s e s = W_s e t := by
+  have h1 : ∀ s ≥ t, (W_s e (s+1)) = (W_s e s) := by
+    intro s h1
+    rw [Ws_eq]
+    simp only [add_tsub_cancel_right, Finset.union_eq_left]
+    have h2 : PhiNew e (s+1) = ∅ := by
+      apply h
+      linarith
+    rw [h2]
+    simp
+  intro s h2
+  induction' s using Nat.strong_induction_on with s ih
+  by_cases h3 : s = t
+  · simp [h3]
+  · have h4 : s - 1 ≥ t := by
+      refine le_sub_one_of_lt ?_
+      exact Nat.lt_of_le_of_ne h2 fun a ↦ h3 (id (Eq.symm a))
+    have h5 : (W_s e (s-1)) = (W_s e t) := by
+      apply ih (s-1)
+      · apply Nat.sub_one_lt
+        cases t
+        · tauto
+        · linarith
+      exact h4
+    rw [← h5]
+    have h6 : s - 1 + 1 = s := by
+      refine Nat.sub_add_cancel ?_
+      cases t
+      · exact one_le_iff_ne_zero.mpr h3
+      · exact one_le_of_lt h2
+    rw [← h6]
+    exact h1 (s - 1) h4
